@prefix odim:    <http://connectdigitalstudy.com/ontology#> .
@prefix connect: <http://connectdigitalstudy.com/ontology#> .
@prefix skos:    <http://www.w3.org/2004/02/skos/core#> .
@prefix rdfs:    <http://www.w3.org/2000/01/rdf-schema#> .

# SKOS: Property Category scheme
odim:PropertyCategoryScheme a skos:ConceptScheme ;
  rdfs:label "Property Category Scheme" ;
  skos:prefLabel "Property categories"@en .

odim:PhysiologicalProperty a skos:Concept ;
  skos:inScheme odim:PropertyCategoryScheme ;
  skos:prefLabel "Physiological"@en ;
  skos:altLabel "Physio"@en ;
  skos:topConceptOf connect:PropertyCategoryScheme ;
  skos:definition "Properties concerning physiological signals and measures (e.g., HR, HRV)."@en .

odim:BehavioralProperty a skos:Concept ;
  skos:inScheme odim:PropertyCategoryScheme ;
  skos:prefLabel "Behavioral"@en ;
  skos:related odim:PhysiologicalProperty ;
  skos:topConceptOf odim:PropertyCategoryScheme ;
  skos:definition "Properties describing human behavior such as activity and sleep."@en .

odim:EnvironmentalProperty a skos:Concept ;
  skos:inScheme odim:PropertyCategoryScheme ;
  skos:prefLabel "Environmental"@en ;
  skos:broader odim:BehavioralProperty ;
  skos:definition "Properties describing environmental context such as light or temperature."@en .

# Scheme top concept links
odim:PropertyCategoryScheme skos:hasTopConcept odim:PhysiologicalProperty , odim:BehavioralProperty .
